# 実験2.1 公理定理を用いた簡単化

## 問題１．f = x' y' z' + x y' z + y' z'

### 簡単化前の論理式
```math
f = x' y' z' + x y' z + y' z'
```

### ブール代数を利用した簡単化

```math
f = x' y' z' + x y' z + y' z'
  = ( x' + x ) y' z + y' z'
  = y' z + y' z'
  = y' ( z + z' )
  = y'
```

### 簡単後の論理式
```math
f = y'
```

## 問題2．f = a' b' + a' b + a b' + a b

### 簡単化前の論理式
```math
f = a' b' + a' b + a b' + a b
```

### ブール代数を利用した簡単化

```math
f = a' b' + a' b + a b' + a b
  = a' ( b' + b ) + a ( b' + b )
  = a' + a
  = 1
```

### 簡単後の論理式
```math
f = 1
```
